\newcommand{\me}{\mathrm{e}}
\newcomman{\md}{\mathrm{d}}
\par\noindent { \bf 06.17 }
\vspace{1cm}

  \bf{06.17} Suppose that $X_1$ and $X_2$ are a random sample of size 2 from a gamma distribution, $X_i\sim\mathrm{GAM}(2,1/2)$.
    \begin{enumerate}
      \item
        Find the pdf of $Y=\sqrt{X_1+X_2}\;;$
      \item
        Find the pdf of $W={X_1}/{X_2}$.
    \end{enumerate}


\begin{proof}[Solution]
  (a) Since $X_1$ and $X_2$ are independent to each other,
  the joint distribution density function is the product of $f(X_1)$ and $f(X_2)$, which is
    $$
      f(X_1,X_2)=
        \begin{cases}
          \left(\frac{1}{\sqrt{2}\;\Gamma(1/2)}\right)^2X_1^{-1/2}X_2^{-1/2}\me^{-(X_1+X_2)\!/2}
          =\frac{1}{2\pi}X_1^{-1/2}X_2^{-1/2}\me^{-(X_1+X_2)/2}, & \mathrm{if}\;X_1,X_2>0; \\
          0, & \mathrm{otherwise}.
        \end{cases}
    $$
  If $x_1=w$, then $x_2=y^2-w$, which implies that
    $$
      J=
        \begin{vmatrix}
          1 & 0 \\
          -1 & 2y
        \end{vmatrix}
      =2y.
    $$
  Now,
    $$
      f(w,y)=
        \begin{cases}
          \frac{1}{\pi}yw^{-1/2}(y^2-w)^{-1/2}\me^{-y^2/2}, & \mathrm{if}\;y^2>w>0; \\
          0, & \mathrm{otherwise}.
        \end{cases}
    $$
  So, since $u=(y^2-w)^{1/2}$ implies that $-2\,\md u=(y^2-w)^{-1/2}\md w$, and $u=y\sin\theta$ implies that $\md u=y\cos\theta \md \theta$,
    \begin{align*}
      f_Y(y)&=\frac{1}{\pi}\int_0^{y^2}y\me^{-y^2/2}w^{-1/2}(y^2-w)^{-1/2}\;\md w \\
      &=\frac{-2}{\pi}\int_y^0y\me^{-y^2/2}(y^2-u^2)^{-1/2}\;\md u \\
      &=\frac{2}{\pi}\int_0^yy\me^{-y^2/2}(y^2-u^2)^{-1/2}\;\md u \\ &=y\me^{-y^2/2}\frac{2}{\pi}\int_0^y\frac{1}{\sqrt{y^2-u^2}}\;\md u\\
      &=y\me^{-y^2/2}\frac{2}{\pi}\int_0^{\pi/2}\frac{y\cos\theta}{\sqrt{y^2-y^2\sin^2\theta}}\;\md \theta\\
      &=y\me^{-y^2/2}\frac{2}{\pi}\int_0^{\pi/2}\md \theta\\
      &=y\me^{-y^2/2}\frac{2}{\pi}\frac{\pi}{2}\\
      &=\begin{cases}
         y\me^{-y^2/2}, & \mathrm{if}\;y>0; \\
          0, & \mathrm{otherwise}.
        \end{cases}
    \end{align*}

  (b) If $X_1=z$,then $X_2=z/w$, which implies that
        $$
      J=
        \begin{vmatrix}
          1 & 0 \\
          1/w & z/w^2
        \end{vmatrix}
      =\frac{z}{w^2}.
    $$
    Now,
    $$
      f(z,w)=
        \begin{cases}
          \frac{1}{2\pi}\frac{z}{w^2}(\frac{z^2}{w})^{-1/2}\,\me^{-(z+z/w)\!/2}, & \mathrm{if}\;z,w>0; \\
          0, & \mathrm{otherwise}.
        \end{cases}
    $$
  So, for getting the marginal density function of $w$, we need to take the integral for the above joint density function with respect to $z$,
    \begin{align*}
     f_W(w)&=\int_0^\infty\frac{1}{2\pi}w^{-3/2}\,\me^{-z(1+1/w)\!/2}\;\md z \\
           &=\left.-\frac{1}{2\pi}\frac{2}{1+1/w}\,\me^{-z(1+1/w)\!/2}w^{-3/2}\,\right|_0^\infty\\
           &=\left.-\frac{1}{\pi(w+1)\sqrt{w}}\,\me^{-z(1+1/w)\!/2}\,\right|_0^\infty\\
           &=\begin{cases}
              \frac{1}{\pi(w+1)\sqrt{w}}, & \mathrm{if}\; w>0; \\
              0, & \mathrm{otherwise}.
     \end{cases}
    \end{align*}
 \end{proof}

